proof that sat is instance of sat'

thys/MFODL_Monitor_Devel/Type_Soundness.thy
@@ -1,568 +1,55 @@
 theory Type_Soundness
   imports Typing
 begin
-context fixes 
-undef_plus :: "event_data \<Rightarrow> event_data \<Rightarrow> event_data" and
-undef_minus :: "event_data \<Rightarrow> event_data \<Rightarrow> event_data" and
-undef_uminus :: " event_data \<Rightarrow> event_data" and
-undef_times :: "event_data \<Rightarrow> event_data \<Rightarrow> event_data" and
-undef_divide :: "event_data \<Rightarrow> event_data \<Rightarrow> event_data" and
-undef_modulo :: "event_data \<Rightarrow> event_data \<Rightarrow> event_data"  and
-undef_double_of_event_data :: "event_data \<Rightarrow> double" and
-undef_integer_of_event_data :: "event_data \<Rightarrow> integer" and
-undef_less_eq :: "event_data \<Rightarrow> event_data \<Rightarrow> bool" and
-undef_eq :: "event_data \<Rightarrow> event_data \<Rightarrow> bool"
-assumes undef_plus_sound:  "\<And>x y. undef_plus (EInt x) (EInt y) = EInt x + EInt y" 
-    "\<And> x y . undef_plus (EFloat x) (EFloat y) = EFloat x + EFloat y"
-assumes undef_minus_sound:  "\<And>x y. undef_minus (EInt x) (EInt y) = EInt x - EInt y" 
-    "\<And> x y . undef_minus (EFloat x) (EFloat y) = EFloat x - EFloat y"
-assumes undef_uminus_sound:  "\<And>x . undef_uminus (EInt x) = - EInt x"
-   "\<And> x. undef_uminus (EFloat x) = - EFloat x "
-assumes undef_times_sound:  "\<And>x y.  undef_times (EInt x) (EInt y) = EInt x * EInt y" 
-    "\<And> x y . undef_times (EFloat x) (EFloat y) = EFloat x * EFloat y"
-assumes undef_divide_sound:  "\<And>x y. undef_divide (EInt x) (EInt y) = EInt x div EInt y" 
-    "\<And> x y .  undef_divide (EFloat x) (EFloat y) = EFloat x div EFloat y"
-assumes undef_modulo_sound:  "\<And>x y.  undef_modulo (EInt x) (EInt y) = EInt x mod EInt y"  
-assumes undef_eq_sound: "\<And>x y.  undef_eq (EInt x) (EInt y) \<longleftrightarrow> EInt x = EInt y"
- "\<And>x y.  undef_eq (EFloat x) (EFloat y) \<longleftrightarrow> EFloat x = EFloat y"
- "\<And> x y. undef_eq (EString x) (EString y) \<longleftrightarrow> EString x = EString y"
 
-assumes undef_double_of_event_data_sound: "\<And>x.  undef_double_of_event_data (EInt x) = double_of_event_data (EInt x)"
-assumes undef_integer_of_event_data_sound: "\<And>x. undef_integer_of_event_data (EFloat x) = integer_of_event_data (EFloat x)"
+interpretation  sat_inst: sat_general "(+)" "(-)" "uminus" "(*)" "(div)" "(mod)" "Event_Data.double_of_event_data" "Event_Data.integer_of_event_data" "(\<le>)"
+  by unfold_locales  auto
 
-assumes undef_less_eq_sound: "\<And>x y. undef_less_eq (EInt x) (EInt y) \<longleftrightarrow> EInt x \<le> EInt y"
- "\<And>x y. undef_less_eq (EFloat x) (EFloat y) \<longleftrightarrow> EFloat x \<le> EFloat y"
- "\<And> x y. undef_less_eq (EString x) (EString y) \<longleftrightarrow> EString x \<le> EString y"
+lemma eval_trm_inst: " sat_inst.eval_trm'  = Formula.eval_trm "
+proof -
+  have  "sat_inst.eval_trm' v f = Formula.eval_trm v f" for v f
+  by (induction f)  auto 
+  then show ?thesis  by auto
+qed 
 
+lemma eval_agg_op_inst: " sat_inst.eval_agg_op' (\<omega>, d) M  = Formula.eval_agg_op (\<omega>, d) M"
+  apply (cases \<omega>)   apply (auto ) apply (induction "flatten_multiset M")  apply (cases \<omega>) apply (auto simp add:  split: list.splits) 
+  apply (smt (verit) foldl_cong min_def sat_inst.undef_min_def sat_inst.undef_min_def) 
+  by (smt (verit) foldl_cong max_def sat_inst.undef_max_def) 
+  
+
+lemma sat_inst_of_sat': "Formula.sat \<sigma> V v i \<phi> = sat_inst.sat' \<sigma> V v i \<phi>"
+ apply (induction \<phi> arbitrary: v V i)  apply  (auto simp add: eval_trm_inst less_event_data_def sat_inst.undef_less_def  split: nat.splits)
+  using eval_trm_inst apply presburger
+                      apply (metis eval_trm_inst) 
+  using eval_agg_op_inst apply presburger+  by  (metis match_cong_strong)+
+
+
+lemma ty_of_sat_safe: "safe_formula \<phi> \<Longrightarrow> S, E \<turnstile> \<phi> \<Longrightarrow> wty_envs S \<sigma> V \<Longrightarrow> 
+  Formula.sat \<sigma> V v i \<phi> \<Longrightarrow> x \<in> Formula.fv \<phi> \<Longrightarrow> Formula.nfv \<phi> \<le> length v \<Longrightarrow> ty_of (v ! x) = E x"
+  using  sat_inst.sat_general_axioms sat_inst_of_sat'
+    sat_general.ty_of_sat'_safe[of  "(+)" "(-)" "uminus" "(*)" "(div)" "(mod)" double_of_event_data integer_of_event_data "(\<le>)"]  
+  by auto  blast
+ 
+
+context sat_general
 begin
 
-definition undef_less :: "event_data \<Rightarrow> event_data \<Rightarrow> bool"  where
-  "undef_less x y \<longleftrightarrow> undef_less_eq x y \<and> \<not> undef_less_eq y x"
-
-definition undef_min :: "event_data \<Rightarrow> event_data \<Rightarrow> event_data" where
-  "undef_min a b = (if undef_less_eq a b then a else b)"
-
-definition undef_max :: "event_data \<Rightarrow> event_data \<Rightarrow> event_data" where
-  "undef_max a b = (if undef_less_eq a b then b else a)"
-
-primrec eval_trm' :: "Formula.env \<Rightarrow> Formula.trm \<Rightarrow> event_data" where
-  "eval_trm' v (Formula.Var x) = v ! x"
-| "eval_trm' v (Formula.Const x) = x"
-| "eval_trm' v (Formula.Plus x y) = undef_plus (eval_trm' v x) ( eval_trm' v y)"
-| "eval_trm' v (Formula.Minus x y) = undef_minus (eval_trm' v x) ( eval_trm' v y)"
-| "eval_trm' v (Formula.UMinus x) = undef_uminus (eval_trm' v x)"
-| "eval_trm' v (Formula.Mult x y) = undef_times (eval_trm' v x) (eval_trm' v y)"
-| "eval_trm' v (Formula.Div x y) = undef_divide (eval_trm' v x) (eval_trm' v y)"
-| "eval_trm' v (Formula.Mod x y) = undef_modulo (eval_trm' v x) (eval_trm' v y)"
-| "eval_trm' v (Formula.F2i x) = EInt (undef_integer_of_event_data (eval_trm' v x))"
-| "eval_trm' v (Formula.I2f x) = EFloat (undef_double_of_event_data (eval_trm' v x))"
-
-
-fun eval_agg_op' :: "Formula.agg_op \<Rightarrow> (event_data \<times> enat) set \<Rightarrow> event_data" where
-  "eval_agg_op' (agg_type.Agg_Cnt, y0) M = (case (flatten_multiset M, finite_multiset M) of
-    (_, False) \<Rightarrow> y0
-    |    ([],_) \<Rightarrow> y0
-    | (xs,_) \<Rightarrow> EInt (integer_of_int (length xs)))"
-| "eval_agg_op' (agg_type.Agg_Min, y0) M = (case  (flatten_multiset M, finite_multiset M) of
-    (_, False) \<Rightarrow> y0
-    |    ([],_) \<Rightarrow> y0
-    | (x # xs,_) \<Rightarrow> foldl undef_min x xs)"
-| "eval_agg_op' (agg_type.Agg_Max, y0) M = (case  (flatten_multiset M, finite_multiset M) of
-    (_, False) \<Rightarrow> y0
-    |    ([],_) \<Rightarrow> y0
-    | (x # xs,_) \<Rightarrow> foldl undef_max x xs)"
-| "eval_agg_op' (agg_type.Agg_Sum, y0) M = (case  (flatten_multiset M, finite_multiset M) of
-    (_, False) \<Rightarrow> y0
-    |    ([],_) \<Rightarrow> y0
-    | (x # xs,_) \<Rightarrow> foldl undef_plus x xs)"
-| "eval_agg_op' (agg_type.Agg_Avg, y0) M =(case  (flatten_multiset M, finite_multiset M) of
-    (_, False) \<Rightarrow> y0
-    |    ([],_) \<Rightarrow> y0
-    | (x#xs,_) \<Rightarrow> EFloat ( undef_double_of_event_data (foldl undef_plus x xs) / double_of_int (length (x#xs))))"
-| "eval_agg_op' (agg_type.Agg_Med, y0) M =(case (flatten_multiset M, finite_multiset M) of
-    (_, False) \<Rightarrow> y0
-    |    ([],_) \<Rightarrow> y0
-    | (xs,_) \<Rightarrow> EFloat (let u = length xs;  u' = u div 2 in
-          if even u then
-            (undef_double_of_event_data (xs ! (u'-1)) + undef_double_of_event_data (xs ! u') / double_of_int 2)
-          else undef_double_of_event_data (xs ! u')))"
-
-fun sat' :: "Formula.trace \<Rightarrow> (Formula.name \<rightharpoonup> nat \<Rightarrow> event_data list set) \<Rightarrow> Formula.env \<Rightarrow> nat \<Rightarrow> 't Formula.formula \<Rightarrow> bool" where
-  "sat' \<sigma> V v i (Formula.Pred r ts) = (case V r of
-       None \<Rightarrow> (r, map (eval_trm' v) ts) \<in> \<Gamma> \<sigma> i
-     | Some X \<Rightarrow> map (eval_trm' v) ts \<in> X i)"
-| "sat' \<sigma> V v i (Formula.Let p \<phi> \<psi>) =
-    sat' \<sigma> (V(p \<mapsto> \<lambda>i. {v. length v = Formula.nfv \<phi> \<and> sat' \<sigma> V v i \<phi>})) v i \<psi>"
-| "sat' \<sigma> V v i (Formula.Eq t1 t2) =  (eval_trm' v t1 = eval_trm' v t2)"
-| "sat' \<sigma> V v i (Formula.Less t1 t2) = undef_less (eval_trm' v t1) (eval_trm' v t2)"
-| "sat' \<sigma> V v i (Formula.LessEq t1 t2) = undef_less_eq (eval_trm' v t1) (eval_trm' v t2)"
-| "sat' \<sigma> V v i (Formula.Neg \<phi>) = (\<not> sat' \<sigma> V v i \<phi>)"
-| "sat' \<sigma> V v i (Formula.Or \<phi> \<psi>) = (sat' \<sigma> V v i \<phi> \<or> sat' \<sigma> V v i \<psi>)"
-| "sat' \<sigma> V v i (Formula.And \<phi> \<psi>) = (sat' \<sigma> V v i \<phi> \<and> sat' \<sigma> V v i \<psi>)"
-| "sat' \<sigma> V v i (Formula.Ands l) = (\<forall>\<phi> \<in> set l. sat' \<sigma> V v i \<phi>)"
-| "sat' \<sigma> V v i (Formula.Exists t \<phi>) = (\<exists>z. sat' \<sigma> V (z # v) i \<phi>)"
-| "sat' \<sigma> V v i (Formula.Agg y \<omega> tys f \<phi>) =
-    (let M = {(x, ecard Zs) | x Zs. Zs = {zs. length zs = length tys \<and> sat' \<sigma> V (zs @ v) i \<phi> \<and> eval_trm' (zs @ v) f = x} \<and> Zs \<noteq> {}}
-    in (M = {} \<longrightarrow> fv \<phi> \<subseteq> {0..< length tys}) \<and> v ! y = eval_agg_op' \<omega> M)"
-| "sat' \<sigma> V v i (Formula.Prev I \<phi>) = (case i of 0 \<Rightarrow> False | Suc j \<Rightarrow> mem I (\<tau> \<sigma> i - \<tau> \<sigma> j) \<and> sat' \<sigma> V v j \<phi>)"
-| "sat' \<sigma> V v i (Formula.Next I \<phi>) = (mem I ((\<tau> \<sigma> (Suc i) - \<tau> \<sigma> i)) \<and> sat' \<sigma> V v (Suc i) \<phi>)"
-| "sat' \<sigma> V v i (Formula.Since \<phi> I \<psi>) = (\<exists>j\<le>i. mem I (\<tau> \<sigma> i - \<tau> \<sigma> j) \<and> sat' \<sigma> V v j \<psi> \<and> (\<forall>k \<in> {j <.. i}. sat' \<sigma> V v k \<phi>))"
-| "sat' \<sigma> V v i (Formula.Until \<phi> I \<psi>) = (\<exists>j\<ge>i. mem I (\<tau> \<sigma> j - \<tau> \<sigma> i) \<and> sat' \<sigma> V v j \<psi> \<and> (\<forall>k \<in> {i ..< j}. sat' \<sigma> V v k \<phi>))"
-| "sat' \<sigma> V v i (Formula.MatchP I r) = (\<exists>j\<le>i. mem I (\<tau> \<sigma> i - \<tau> \<sigma> j) \<and> Regex.match (sat' \<sigma> V v) r j i)"
-| "sat' \<sigma> V v i (Formula.MatchF I r) = (\<exists>j\<ge>i. mem I (\<tau> \<sigma> j - \<tau> \<sigma> i) \<and> Regex.match (sat' \<sigma> V v) r i j)"
-
-
-
-lemma eval_trm_sound: 
-  assumes "E \<turnstile> f :: t"  "\<forall>y\<in>fv_trm f. ty_of (v ! y) = E y"
-  shows "Formula.eval_trm v f = eval_trm' v f"
-  using assms  
-  apply  (induction  rule: wty_trm.induct) apply (auto simp add: numeric_ty_def)
-  subgoal for x y  using  value_of_eval_trm[of E x v] value_of_eval_trm[of E y v] by (auto simp add: undef_plus_sound)
-    subgoal for x y  using  value_of_eval_trm[of E x v] value_of_eval_trm[of E y v] by (auto simp add: undef_plus_sound)
-  subgoal for x y
-    using  value_of_eval_trm[of E x v] value_of_eval_trm[of E y v] by (auto simp add: undef_minus_sound) 
- subgoal for x y
-   using  value_of_eval_trm[of E x v] value_of_eval_trm[of E y v] by (auto simp add: undef_minus_sound)
- subgoal for x 
-   using  value_of_eval_trm[of E x v]  by (auto simp add: undef_uminus_sound)
- subgoal for x 
-   using  value_of_eval_trm[of E x v]  by (auto simp add: undef_uminus_sound)
-  subgoal for x y  using  value_of_eval_trm[of E x v] value_of_eval_trm[of E y v] by (auto simp add: undef_times_sound)
-  subgoal for x y  using  value_of_eval_trm[of E x v] value_of_eval_trm[of E y v] by (auto simp add: undef_times_sound)
-  subgoal for x y  using  value_of_eval_trm[of E x v] value_of_eval_trm[of E y v] by (auto simp add: undef_divide_sound)
-  subgoal for x y  using  value_of_eval_trm[of E x v] value_of_eval_trm[of E y v] by (auto simp add: undef_divide_sound)
-  subgoal for x y  using  value_of_eval_trm[of E x v] value_of_eval_trm[of E y v] by (auto simp add: undef_modulo_sound)
-  subgoal for x  using  value_of_eval_trm[of E x v] by (auto simp add: undef_integer_of_event_data_sound)
-  subgoal for x  using  value_of_eval_trm[of E x v] by (auto simp add: undef_double_of_event_data_sound)
-  done
-
-lemma nfv_exists: " Formula.nfv \<phi> \<le> Suc (Formula.nfv (Formula.Exists t \<phi>))"
-   apply (auto simp add: Formula.nfv_def fvi_Suc) 
-  by (metis Max.coboundedI finite_fvi finite_imageI finite_insert fvi_Suc imageI insertCI list_decode.cases)
-
-lemma match_sat'_fv: assumes "safe_regex temp Strict r"
-    "Regex.match (sat' \<sigma> V v) r j i"
-    "x \<in> fv (formula.MatchP I r) \<or> x \<in>fv (formula.MatchF I r)"
-  shows "\<exists>\<phi>\<in>atms r. \<exists>k. sat' \<sigma> V v k \<phi> \<and> x \<in> fv \<phi>"
-  using assms
-  proof (induction r arbitrary:i j)
-
-    case (Plus r1 r2)
-  moreover obtain k where "\<exists>j. Regex.match (sat' \<sigma> V v) r1 j k \<or>  Regex.match (sat' \<sigma> V v) r2 j k" using  Plus.prems(2)  by auto
-  moreover {
-    assume assm: "\<exists>j. Regex.match (sat' \<sigma> V v) r1 j k"
-    then have ?case using Plus.prems(1,3) Plus.IH(1)  by (fastforce simp add: atms_def) 
-  } moreover {
-    assume assm: "\<exists>j. Regex.match (sat' \<sigma> V v) r2 j k"
-    from this have ?case using Plus.prems(1,3) Plus.IH(2) by (fastforce simp add: atms_def)
-  }
-  ultimately show ?case by auto
-next
-  case (Times r1 r2)
-  then show ?case  using Times.prems match_le Times.IH  by (cases temp) fastforce+
-qed  auto
-
-
-
-lemma ty_of_sat'_safe: "safe_formula \<phi> \<Longrightarrow> S, E \<turnstile> \<phi> \<Longrightarrow> wty_envs S \<sigma> V \<Longrightarrow> 
-  sat' \<sigma> V v i \<phi> \<Longrightarrow> x \<in> Formula.fv \<phi> \<Longrightarrow> Formula.nfv \<phi> \<le> length v \<Longrightarrow> ty_of (v ! x) = E x"
-proof (induction arbitrary: S E V v i x rule: safe_formula_induct)
-  case (Eq_Const c d)
-  then show ?case by auto
-next
-  case (Eq_Var1 c xa)
-   case (Eq_Var1 c xa)
-  from Eq_Var1.prems(1) obtain t where 
-" E \<turnstile> (trm.Const c) :: t" and "E \<turnstile> (trm.Var xa) :: t"
-    by cases
-  from Eq_Var1(4)  have "x = xa" by auto
-  from this `E \<turnstile> (trm.Var xa) :: t` have "E x = t" using  wty_trm.cases by fastforce
-  from this Eq_Var1 ` E \<turnstile> (trm.Const c) :: t` show ?case
-    by (metis \<open>x = xa\<close> empty_iff eval_trm'.simps(1) fvi_trm.simps(2) sat'.simps(3) eval_trm_sound ty_of_eval_trm)
-
-next
-  case (Eq_Var2 c xa)
-    from Eq_Var2.prems(1) obtain t where 
-" E \<turnstile> (trm.Const c) :: t" and "E \<turnstile> (trm.Var xa) :: t"
-    by cases
-  from Eq_Var2(4)  have "x = xa" by auto
-  from this `E \<turnstile> (trm.Var xa) :: t` have "E x = t" using  wty_trm.cases by fastforce
-  from this Eq_Var2 ` E \<turnstile> (trm.Const c) :: t` show ?case
-    by (metis \<open>x = xa\<close> empty_iff eval_trm'.simps(1) fvi_trm.simps(2) sat'.simps(3) eval_trm_sound ty_of_eval_trm)
-  
-next
-  case (neq_Var xa)
-  thus ?case by (auto) 
-next
-  case (Pred p tms)
-  from Pred.prems(1) obtain tys where
-    S_p: "S p = Some tys" and
-    xs_ts: "list_all2 (\<lambda>tm ty. E \<turnstile> tm :: ty) tms tys"
-    by cases
-  let ?xs = "map (eval_trm' v) tms"
-  have wty_xs: "wty_tuple tys ?xs"
-  proof (cases "p \<in> dom V")
-    case True
-    then have "?xs \<in> the (V p) i"
-      using Pred.prems(3) by auto
-    with True show ?thesis
-      using Pred.prems(2) by (auto simp: S_p dest!: wty_envs_V_D)
-  next
-    case False
-    then have "(p, ?xs) \<in> \<Gamma> \<sigma> i"
-      using Pred.prems(3) by (auto split: option.splits)
-    with False show ?thesis
-      using Pred.prems(2) by (auto simp: S_p dest!: wty_envs_\<Gamma>_D)
-  qed
-  from Pred obtain k where k: "k < length tms" "tms ! k = Formula.Var x"
-    by (fastforce simp: trm.is_Var_def trm.is_Const_def in_set_conv_nth)
-  with Pred.prems have "v ! x = ?xs ! k" by simp
-  with wty_xs k have "ty_of (v ! x) = tys ! k"
-    by (auto simp: wty_tuple_def list_all2_conv_all_nth)
-  also have "\<dots> = E x"
-    using xs_ts k
-    by (fastforce simp: list_all2_conv_all_nth elim: wty_trm.cases)
-  finally show ?case .
-next
-  case (Let p \<phi> \<psi>)
-  let ?V' = "V(p \<mapsto> \<lambda>i. {v. length v = Formula.nfv \<phi> \<and> sat' \<sigma> V v i \<phi>})"
-  from Let.prems(1) obtain E' where
-    wty_\<phi>: "S, E' \<turnstile> \<phi>" and
-    wty_\<psi>: "S(p \<mapsto> tabulate E' 0 (Formula.nfv \<phi>)), E \<turnstile> \<psi>"
-    by (cases pred: wty_formula)
-  let ?tys = "tabulate E' 0 (Formula.nfv \<phi>)"
-  {
-    fix v' i
-    assume "length v' = Formula.nfv \<phi>" and "sat' \<sigma> V v' i \<phi>"
-    then have "wty_tuple ?tys v'"
-      using Let.IH(1) wty_\<phi> Let.prems(2) Let.hyps(1)
-      by (auto simp: wty_tuple_def list_all2_conv_all_nth)
-  }
-  with Let.prems(2) have "wty_envs (S(p \<mapsto> ?tys)) \<sigma> ?V'"
-    by (auto simp: wty_envs_def wty_event_def)
-  from Let.prems(3) have "sat' \<sigma> ?V' v i \<psi>" by simp
-  from Let.prems(4) have "x \<in> fv \<psi>" by simp
-  from Let have "Formula.nfv \<psi> \<le> length v" by auto
-  show ?case by (rule Let.IH(2)) fact+
-next
-  case (And_assign \<phi> \<psi>)
-  from And_assign.prems(1) have phi1: "S, E \<turnstile> \<phi>" by cases
-  from And_assign.prems(3) have phi2: "sat' \<sigma> V v i \<psi>" by auto
-  from And_assign.prems(4) have "x \<in> fv \<phi> \<or> x \<in> fv \<psi>" by auto
-  from this show ?case
-  proof cases
-    assume "x \<in> fv \<phi>"
-    from this And_assign phi1 phi2 show ?case by auto
-  next
-    assume x_not_\<phi>: "x \<notin> fv \<phi>"
-    from this And_assign.prems(4) have "x \<in> fv \<psi>" by auto
-    from And_assign.hyps(2) obtain a b where \<psi>_eq: "\<psi> = Formula.Eq a b"
-      by (auto simp: safe_assignment_def split: formula.splits)
-    moreover {
-      assume a_def: "a = Formula.Var x"
-      from this  x_not_\<phi> have fvb: "fv_trm b \<subseteq> fv \<phi>" using And_assign(2) by  (auto simp: safe_assignment_def \<psi>_eq split: trm.splits) 
-      have eval:" v! x = eval_trm' v b" using And_assign(6) a_def \<psi>_eq by auto
-      have Ebx: "E \<turnstile> b :: E  x"  using And_assign(4) by (auto simp: \<psi>_eq a_def elim: wty_trm.cases wty_formula.cases)
-      have "(\<lambda>y. ty_of (v ! y)) \<turnstile> b :: E x" apply (rule  iffD1[OF wty_trm_fv_cong,OF _ Ebx]) apply (subst eq_commute) 
-        apply (rule And_assign(3)) using And_assign fvb by (auto elim: wty_formula.cases) 
-      then have ?case using ty_of_eval_trm unfolding eval
-        using And_assign(4) by (auto simp: \<psi>_eq a_def eval_trm_sound elim: wty_formula.cases)
-    }
-    moreover {
-     assume a_def: "b = Formula.Var x"
-      from this  x_not_\<phi> have fvb: "fv_trm a \<subseteq> fv \<phi>" using And_assign(2) by  (auto simp: safe_assignment_def \<psi>_eq split: trm.splits) 
-      have eval:" v! x = eval_trm' v a" using And_assign(6) a_def \<psi>_eq by auto
-      have Ebx: "E \<turnstile> a :: E  x"  using And_assign(4) by (auto simp: \<psi>_eq a_def elim: wty_trm.cases wty_formula.cases)
-      have "(\<lambda>y. ty_of (v ! y)) \<turnstile> a :: E x" apply (rule  iffD1[OF wty_trm_fv_cong,OF _ Ebx]) apply (subst eq_commute) 
-        apply (rule And_assign(3)) using And_assign fvb by (auto elim: wty_formula.cases) 
-      then have ?case using ty_of_eval_trm unfolding eval
-        using And_assign(4)  by (auto simp: \<psi>_eq a_def eval_trm_sound elim: wty_formula.cases)
-    }
-    moreover
-      have "a = Formula.Var x \<or> b = Formula.Var x" using And_assign(2) And_assign(7) x_not_\<phi> by (auto simp: \<psi>_eq safe_assignment_def split: Formula.trm.splits) 
-    ultimately show ?case by auto
-qed
- next
-  case (And_safe \<phi> \<psi>)
-  from And_safe.prems(1) obtain "S, E \<turnstile> \<phi>" and "S, E \<turnstile> \<psi>" by cases
-  from And_safe.prems(3) have "sat' \<sigma> V v i \<phi>" and "sat' \<sigma> V v i \<psi>"
-    by simp_all
-  from And_safe.prems(4) consider (in_\<phi>) "x \<in> fv \<phi>" | (in_\<psi>) "x \<in> fv \<psi>" by auto
-  then show ?case
-  proof cases
-    case in_\<phi>
-  from And_safe have "Formula.nfv \<phi> \<le> length v" by auto
-    show ?thesis by (rule And_safe.IH(1)) fact+
-  next
-    case in_\<psi>
-  from And_safe have "Formula.nfv \<psi> \<le> length v" by auto
-    show ?thesis by (rule And_safe.IH(2)) fact+
-  qed
-next
-  case (And_constraint \<phi> \<psi>)
-  have xfree: "x \<in> fv \<phi>" using And_constraint(4) And_constraint(10) by auto
-  from And_constraint(7) have "S, E \<turnstile> \<phi>" by cases
-  from this xfree And_constraint(6,8-9,11) show ?case by auto
-next
-  case (And_Not \<phi> \<psi>)
-  from And_Not.prems(4) And_Not.hyps(4) have xfree: "x \<in> fv \<phi>" by auto
-  from And_Not.prems(1) have "S, E \<turnstile> \<phi>" by cases
-  from this xfree And_Not  show ?case by auto 
-next
-  case (Ands l pos neg)
-  from Ands have "\<exists>\<phi> \<in> set l . x \<in> fv \<phi>" by auto
-  from this obtain \<psi> where psidef: "\<psi> \<in> set l \<and> x \<in> fv \<psi>" by blast
-  from this have "\<exists>\<phi>\<in>set pos. x \<in>fv  \<phi>" 
-  proof cases
-    assume "safe_formula \<psi>"
-    then have "\<psi> \<in> set pos" using Ands(1) by (auto simp add: psidef)
-    thus "\<exists>\<phi>\<in>set pos. x \<in>fv  \<phi>" using psidef by auto
-  next
-    assume " \<not> safe_formula \<psi>"
-    then have "\<psi> \<in> set neg" using Ands(1) by (auto simp add: psidef)
-    thus "\<exists>\<phi>\<in>set pos. x \<in>fv  \<phi>" using Ands(1) Ands(5) psidef by auto
-  qed
-  from this obtain \<phi> where phidef: "\<phi> \<in> set pos \<and> x \<in> fv \<phi>" by blast
-  from this Ands(1) have phi_in_l: "\<phi> \<in> set l" by auto
-  from phidef Ands(6) have phi_IH: "S, E \<turnstile> \<phi> \<Longrightarrow>
-    wty_envs S \<sigma> V \<Longrightarrow>
-    sat' \<sigma> V v i \<phi> \<Longrightarrow> x \<in> fv \<phi> \<Longrightarrow> Formula.nfv \<phi> \<le> length v \<Longrightarrow> ty_of (v ! x) = E x"
-        using list_all2_iff by (smt (verit, ccfv_SIG) Ball_set_list_all)
-      from Ands.prems(1) have  "\<forall>\<phi> \<in> set l. S, E \<turnstile> \<phi>" by cases
-      from this phi_in_l have p1: "S, E \<turnstile> \<phi>"  by auto
-      from phi_in_l Ands.prems(3) have p3: "sat' \<sigma> V v i \<phi>" by auto
-      from phi_in_l Ands have p5: "Formula.nfv \<phi> \<le> length v" by auto
-  from  phi_IH p1 Ands.prems(2) p3 phidef p5  show ?case by auto
-next
-  case (Neg \<phi>)
-  from Neg show ?case by auto
-next
-  case (Or \<phi> \<psi>)
-  from Or.prems(3) have " (sat' \<sigma> V v i \<phi>) \<or>( sat' \<sigma> V v i \<psi>)" by auto
-  from this show ?case 
-  proof
-    assume assm: "(sat' \<sigma> V v i \<phi>)"
-  from Or(1) Or.prems(4) have xfv: "x \<in> fv \<phi>" by auto
-  from Or.prems(1) have "S, E \<turnstile> \<phi>" by cases
-  from this assm Or.prems(2,3) Or(4) Or.prems(5) xfv show ?case by auto
-next 
-  assume assm: "( sat' \<sigma> V v i \<psi>)"
- from Or(1) Or.prems(4) have xfv: "x \<in> fv \<psi>" by auto
-  from Or.prems(1) have "S, E \<turnstile> \<psi>" by cases
-  from this assm Or.prems(2,3) Or(5) Or.prems(5) xfv show ?case by auto
-qed
-next
-  case (Exists \<phi>)
-  from Exists.prems(1) obtain t where "S, case_nat t E \<turnstile> \<phi>" by cases
-  from Exists.prems(3) obtain z where "sat' \<sigma> V (z#v) i \<phi>" by auto
-  from Exists.prems(4) have "Suc x \<in> fv \<phi>" by (simp add: fvi_Suc)
-  from Exists have "Formula.nfv \<phi> \<le> Suc (length v)" apply (auto simp add: Formula.nfv_def)
-    by (metis fvi_Suc le0 old.nat.exhaust)
-
-  have "ty_of ((z#v) ! Suc x) = case_nat t E (Suc x)"
-    by (rule Exists.IH) (simp?, fact)+
-  then show ?case by simp
-next
-  case (Agg y \<omega> tys f \<phi>)
- have "\<forall>z \<in>Formula.fvi (length tys) \<phi>. Suc z \<le> length v " using Agg.prems(5) by (auto simp add: Formula.nfv_def)
-    from this have "\<forall>z \<in>Formula.fv \<phi>. Suc z - length tys \<le> length v "  using  fvi_iff_fv  nat_le_linear 
-      by (metis Suc_diff_le diff_add diff_is_0_eq' diff_zero not_less_eq_eq) 
-    from this have nfv_tys_v: "Formula.nfv \<phi> \<le> length tys + length v" by (auto simp add: Formula.nfv_def)
-
-  have case_split:" x \<in> Formula.fvi (length tys) \<phi> \<or> x \<in> Formula.fvi_trm (length tys) f \<or> x = y" using Agg.prems(4) by auto
- 
-  moreover {
-    assume asm: "x \<in> Formula.fvi (length tys) \<phi>"
-    from this have "\<not> fv \<phi> \<subseteq> {0..< length tys}" using fvi_iff_fv[of x "length tys" \<phi>] by auto
-    from this have M: "{(x, ecard Zs) | 
-  x Zs. Zs = {zs. length zs = length tys \<and> sat' \<sigma> V (zs @ v) i \<phi> \<and> eval_trm' (zs @ v) f = x} \<and> Zs \<noteq> {}} \<noteq> {}" using Agg.prems(3) by auto
-    from this obtain zs where sat: "sat' \<sigma> V (zs @ v) i \<phi> \<and> length zs = length tys" by auto
-    from nfv_tys_v have nfv: "Formula.nfv \<phi> \<le> length (zs @ v)"  by (auto simp add: sat)
-    have "ty_of ((zs@v) ! (x + length tys)) = agg_env E tys (x + length tys)"
-      apply (rule Agg.IH[of \<phi> S "agg_env E tys" V "zs @ v" i "x+ length tys"]) using Agg.prems(1) Agg(4) sat asm nfv Agg.prems(1-2) fvi_iff_fv
-      by (auto elim: wty_formula.cases)
-    from this have ?case apply (auto simp add: agg_env_def) by (metis add.commute nth_append_length_plus sat)
-  } 
-  moreover {
-    assume "x \<notin> Formula.fvi (length tys) \<phi>"
-    from this have eq: "x = y" using Agg(3) case_split fvi_iff_fv fvi_trm_iff_fv_trm by blast
-    obtain d agg_type where omega_def: "\<omega> = (agg_type, d)" using surjective_pairing by blast
-    from Agg.prems(1) this have  "\<exists>t .E y = t_res agg_type t" by cases auto
-    from this eq obtain t where t_def: "E x = t_res agg_type t" by blast
-    from  Agg.prems(1) have
- ty_of_d: "ty_of d = t_res agg_type t" apply cases using eq omega_def t_def by auto
-    from Agg.prems(3) eq obtain M where  M_def: "M = {(x, ecard Zs) | x Zs. Zs = {zs. length zs = length tys \<and> sat' \<sigma> V (zs @ v) i \<phi>
-        \<and> eval_trm' (zs @ v) f = x} \<and> Zs \<noteq> {}} \<and> v!x = eval_agg_op' \<omega> M" by auto
-   
-        {
-           assume finite_M: "finite_multiset M"
-    from this   have finite_set:"finite {x. {zs. length zs = length tys \<and> sat' \<sigma> V (zs @ v) i \<phi> \<and> eval_trm' (zs @ v) f = x} \<noteq> {}}"
-       using finite_fst by (auto simp add: finite_multiset_def M_def ) 
-    have flatten: "set (flatten_multiset M) \<subseteq> fst ` M" using finite_set  set_of_flatten_multiset[of M
- "(\<lambda>x . {zs . length zs = length tys \<and> sat' \<sigma> V (zs @ v) i \<phi> \<and> eval_trm' (zs @ v) f = x} )"]
-       by (auto simp add:  M_def) 
-    from this  have evaltrm: "z \<in> set (flatten_multiset M) \<Longrightarrow>  \<exists> zs. length zs = length tys \<and> sat' \<sigma> V (zs @ v) i \<phi> \<and> eval_trm' (zs @ v) f = z" 
-      for z using  M_def by (auto simp add: image_def)
-     have th2: ?case if minmaxsum: "agg_type = agg_type.Agg_Min \<or> agg_type = agg_type.Agg_Max \<or> agg_type = agg_type.Agg_Sum" and alist_def: " flatten_multiset
-     {(x, ecard {zs. length zs = length tys \<and> sat' \<sigma> V (zs @ v) i \<phi> \<and> eval_trm' (zs @ v) f = x}) |x.
-      \<exists>xa. sat' \<sigma> V (xa @ v) i \<phi> \<and> length xa = length tys \<and> eval_trm' (xa @ v) f = x} =
-    a # list"  for a list
-     proof -
-      have ty_of_list: "z=a \<or> z \<in> set list \<Longrightarrow> \<exists>zs .ty_of (eval_trm' (zs @ v) f) = t \<and> ty_of z = t" for z
-      proof -
-          assume z_def: "z=a \<or> z \<in> set list"
-        from z_def obtain zs where zs_def: " length zs = length tys \<and> sat' \<sigma> V (zs @ v) i \<phi> \<and> eval_trm' (zs @ v) f = z" using alist_def evaltrm M_def by auto
-        from Agg.prems(1) have wty_f: " agg_env E tys  \<turnstile> f :: t" apply cases  using omega_def t_def minmaxsum eq  by auto  
-        have fv_ty:"\<forall>y\<in>fv_trm f. ty_of ((zs @ v) ! y) = agg_env E tys y"
-        proof 
-          fix y
-          assume assm: "y \<in> fv_trm f"
-          have  sat: "sat' \<sigma> V (zs @ v) i \<phi>"  using zs_def by auto 
-          show "ty_of ((zs @ v) ! y) = agg_env E tys y" using zs_def assm Agg(3,4) Agg.prems(1-2) nfv_tys_v sat  Agg.IH[of \<phi> S "agg_env E tys" V "zs@v" i y]
-            by (auto elim: wty_formula.cases)
-        qed      
-        have ty_of_z: "ty_of (eval_trm' (zs @ v) f) = t" using wty_f fv_ty   ty_of_eval_trm[of "agg_env E tys" f t "zs@v" ]
-          by (auto simp add: eval_trm_sound)
-        from this zs_def show  ?thesis by auto
-      qed 
-      from this obtain zs where zs_def: "ty_of (eval_trm' (zs @ v) f) = t" by auto
-      from ty_of_list have indass: "ty_of a = t \<and> (\<forall>z \<in> set list . ty_of z = t)" by auto
-     
-      from this have foldl_evaltrm: "foldfun = min \<or> foldfun = max
-        \<Longrightarrow> ty_of (foldl foldfun a list) = ty_of (eval_trm' (zs @ v) f)" for foldfun using indass 
-          proof  (induction list arbitrary: a foldfun)
-            case Nil
-            then show ?case using zs_def by auto
-          next
-            case (Cons aa tail)
-             have minmax: " ty_of (foldl foldfun (foldfun a aa) tail) = ty_of (eval_trm' (zs @ v) f)"
-              using Cons.IH[of _ "foldfun a aa"] Cons apply auto 
-               apply (metis min_def) by (metis max_def) 
-              then show ?case by auto
-            qed
-
-          from indass have foldl_evaltrm_Sum: 
-              "t \<in> numeric_ty \<Longrightarrow> ty_of (foldl undef_plus a list) = ty_of (eval_trm' (zs@v) f)" 
-              proof (induction list arbitrary: a)
-                  case (Cons aa tail)
-                  from this have "ty_of (undef_plus a aa) = t"  apply (cases aa)  apply ( auto simp add: numeric_ty_def ty_of_plus)
-                     apply (cases a) apply (auto simp add: undef_plus_sound)
-                    by (cases a)(auto simp add: undef_plus_sound)
-
-                  then show ?case using Cons.prems(1) Cons.IH[of "undef_plus a aa"] apply auto 
-                    by (metis Cons.prems(2) list.set_intros(2))
-                qed (auto simp add: zs_def)
-
- from indass have foldl_evaltrm_Min: 
-              " ty_of (foldl undef_min a list) = t" 
-              proof (induction list arbitrary: a)
-                  case (Cons aa tail)
-            from this have "ty_of (undef_min a aa) = t"  apply (cases aa) by ( auto simp add: numeric_ty_def undef_min_def undef_less_eq_sound)
-                  then show ?case using Cons.prems(1) Cons.IH[of "undef_min a aa"] by auto 
-                qed auto
-
- from indass have foldl_evaltrm_Max: 
-              " ty_of (foldl undef_max a list) = t" 
-              proof (induction list arbitrary: a)
-                  case (Cons aa tail)
-            from this have "ty_of (undef_max a aa) = t"  apply (cases aa) by ( auto simp add: numeric_ty_def undef_max_def undef_less_eq_sound)
-                  then show ?case using Cons.prems(1) Cons.IH[of "undef_max a aa"] by auto 
-              qed auto
-           from Agg.prems(1) t_def eq omega_def have num_ty: "agg_type = agg_type.Agg_Sum \<Longrightarrow> t \<in> numeric_ty" by cases auto
-         
-    
-            from  num_ty  finite_M foldl_evaltrm foldl_evaltrm_Sum foldl_evaltrm_Min foldl_evaltrm_Max show  ?thesis apply (cases agg_type)
-               by (auto simp add: M_def  alist_def omega_def finite_multiset_def   
-                      t_def zs_def   split: list.splits) 
-   
-         qed
-          from  finite_M th2  M_def t_def omega_def  have ?case apply (cases agg_type) 
-            by (auto simp add: ty_of_d split: list.splits)        
-        }
-        moreover{
-             assume not_finite: "\<not> finite_multiset M"
-         from this t_def  M_def  omega_def have  ?case apply (cases agg_type)
-                by ( auto simp add: ty_of_d split: list.splits) 
-         }
-         ultimately have ?case by auto 
-     
-  } 
-  ultimately show ?case by auto
-next
-  
-  case (Prev I \<phi>)
-   from Prev.prems(1) have wty: "S, E \<turnstile> \<phi>" by cases
-  from Prev.prems(3) have forall_j: "\<forall>j . i = Suc j \<longrightarrow> sat' \<sigma> V v j \<phi>" by auto
-  from this have "sat' \<sigma> V v (Nat.pred i) \<phi>" using Prev.prems by (auto split: nat.splits)
-  from this wty Prev.prems(2-5) Prev.IH show ?case by auto
-next
-  case (Next I \<phi>)
-  from Next.prems(1,2-5) Next.IH show ?case by (auto elim: wty_formula.cases)
-next
-  case (Since \<phi> I \<psi>)
-  from Since(1,9) have xfv: "x \<in> fv \<psi>" by auto
-  from this  Since.prems(1,2-5) Since.IH show ?case by (auto elim: wty_formula.cases)
-next
-  case (Not_Since \<phi> I \<psi>)
-  from Not_Since.prems(1) have wty: "S, E \<turnstile> \<psi>" by cases
-  from Not_Since(1,10) have xfv: "x \<in> fv \<psi>" by auto
-  from this wty Not_Since.prems(2-5) Not_Since.IH show ?case by auto
-next
-  case (Until \<phi> I \<psi>)
-  from Until(1,9) have xfv: "x \<in> fv \<psi>" by auto
-  from this  Until.prems(1,2-5) Until.IH show ?case by (auto elim: wty_formula.cases)
-next
-  case (Not_Until \<phi> I \<psi>)
- from Not_Until.prems(1) have wty: "S, E \<turnstile> \<psi>" by cases
-  from Not_Until(1,10) have xfv: "x \<in> fv \<psi>" by auto
-  from this wty Not_Until.prems(2-5) Not_Until.IH show ?case by auto
-next
-  case (MatchP I r)
-  from MatchP.prems(3) have "(\<exists>j. Regex.match (sat' \<sigma> V v) r j i)" by auto
-    from this  MatchP(1)  MatchP.prems(4) obtain \<phi> j where phidef: " \<phi> \<in> atms r" " sat' \<sigma> V v j \<phi>" "x \<in> fv \<phi> " using match_sat'_fv  by auto blast
-    have "\<forall>a \<in> fv \<phi>. a \<in> fv_regex r" using   phidef(1)  apply (induction r) apply auto 
-      subgoal for \<psi>  apply (cases "safe_formula \<psi>") apply auto by (cases \<psi>) auto 
-      done
-    from  this MatchP.prems(4,5) phidef  have nfv: "Formula.nfv \<phi> \<le> length v"  by  (auto simp add: Formula.nfv_def)
-    from MatchP.IH MatchP.prems have IH: "S, E \<turnstile> \<phi> \<Longrightarrow>\<phi> \<in> atms r \<Longrightarrow>
-     sat' \<sigma> V v j \<phi> \<Longrightarrow> x \<in> fv \<phi> \<Longrightarrow> Formula.nfv \<phi> \<le> length v \<Longrightarrow> ty_of (v ! x ) = E x"
-    for \<phi> E  v  x by blast
-   from MatchP.prems(1) MatchP(1) have  "S, E \<turnstile> \<phi>" using  Regex.Regex.regex.pred_set[of "(\<lambda>\<phi>. S, E \<turnstile> \<phi>)"] phidef(1) wty_regexatms_atms  by cases auto
-  then show ?case apply (rule IH) using nfv  MatchP.prems(5) phidef by auto
- 
-next
-  case (MatchF I r)
- from MatchF.prems(3) have "(\<exists>j. Regex.match (sat' \<sigma> V v) r  i j)" by auto
-    from this  MatchF(1)  MatchF.prems(4) obtain \<phi> j where phidef: " \<phi> \<in> atms r" " sat' \<sigma> V v j \<phi>" "x \<in> fv \<phi> " using match_sat'_fv  by auto blast
-    have "\<forall>a \<in> fv \<phi>. a \<in> fv_regex r" using   phidef(1)  apply (induction r) apply auto 
-      subgoal for \<psi>  apply (cases "safe_formula \<psi>") apply auto by (cases \<psi>) auto 
-      done
-    from  this MatchF.prems(4,5) phidef  have nfv: "Formula.nfv \<phi> \<le> length v"  by  (auto simp add: Formula.nfv_def)
-    from MatchF.IH MatchF.prems have IH: "S, E \<turnstile> \<phi> \<Longrightarrow>\<phi> \<in> atms r \<Longrightarrow>
-     sat' \<sigma> V v j \<phi> \<Longrightarrow> x \<in> fv \<phi> \<Longrightarrow> Formula.nfv \<phi> \<le> length v \<Longrightarrow> ty_of (v ! x ) = E x"
-    for \<phi> E  v  x by blast
-    from MatchF.prems(1) MatchF(1) have  "S, E \<turnstile> \<phi>" using  Regex.Regex.regex.pred_set[of "(\<lambda>\<phi>. S, E \<turnstile> \<phi>)"] phidef(1) wty_regexatms_atms  by cases auto
-  then show ?case apply (rule IH) using nfv  MatchF.prems(5)  phidef by auto
-
-qed
-
-
 lemma soundness:
-  assumes  "S,E \<turnstile> \<phi>" "\<forall>y\<in>fv \<phi>. ty_of (v ! y) = E y" "safe_formula \<phi>" "wty_envs S \<sigma> V"
+  assumes   "S,E \<turnstile> \<phi>" "\<forall>y\<in>fv \<phi>. ty_of (v ! y) = E y" "safe_formula \<phi>"  "wty_envs S \<sigma> V"
    "Formula.nfv \<phi> \<le> length v"
-  shows "Formula.sat \<sigma> V v i \<phi> \<longleftrightarrow> sat' \<sigma> V v i \<phi>" 
+ shows "Formula.sat \<sigma> V v i \<phi> \<longleftrightarrow> sat' \<sigma> V v i \<phi>" 
+
  using assms  proof (induction S E \<phi>  arbitrary: v V i rule: wty_formula.induct)
-  
+
   case (Pred S p tys E tms )
   from  Pred  have tms_wty: "x \<in> set tms \<Longrightarrow> \<exists>t \<in> set tys. E \<turnstile> x :: t " for x by (metis Pred.hyps(2) in_set_conv_nth list_all2_conv_all_nth)
    have eval_tms_eq: "map (Formula.eval_trm v) tms = map (eval_trm' v) tms" using  tms_wty Pred(3) apply auto
      subgoal for x using eval_trm_sound[of E x _ v] by auto done
   then show ?case apply auto by (metis eval_tms_eq )+
 next
-  case (Eq E x1 t x2)
-   from Eq show ?case using eval_trm_sound  ty_of_eval_trm  value_of_eval_trm[of E x2 v  ] value_of_eval_trm[of E x1 v  ]
-    by (cases t) (auto simp add: undef_eq_sound) 
+  case (Eq E x t y S)
+  then show ?case using eval_trm_sound by auto 
 next
   case (Less E x1 t x2)
   then show ?case using eval_trm_sound  ty_of_eval_trm value_of_eval_trm[of E x2 v  ] value_of_eval_trm[of E x1 v  ] 
@@ -591,9 +78,20 @@ next
 
   then show ?case using Let by auto
 next
-  find_theorems nth length
   case (Agg E y agg_type t tys f S \<phi> d)
   then show ?case  apply auto sorry
+
+next
+  case (Neg S E \<phi>)
+  from Neg.prems(2) have "safe_formula \<phi>" apply (cases \<phi>) apply auto sorry
+  then show ?case sorry
+
+next
+  case (And S E \<phi> \<psi>)
+  then show ?case sorry
+next
+  case (Ands \<phi>s S E)
+  then show ?case sorry
 next
   case (Exists S t E \<phi> )
    {
@@ -618,19 +116,105 @@ next
     from this have " Formula.sat \<sigma> V (za # v) i \<phi>" using Exists.IH[of "za#v" V i] Exists(4-6) nfv_exists[of \<phi> t] assm by auto
   }
   ultimately show ?case   by auto 
+
 next
+
+  case (Since S E \<phi> \<psi> \<I>)
+  then show ?case sorry
+next
+  case (Until S E \<phi> \<psi> \<I>)
+  then show ?case sorry
+next
+
   case (MatchF S E x2 x1) 
   from this  have other_IH: "\<phi> \<in> regex.atms x2 \<Longrightarrow> Formula.sat \<sigma> V5 v i5 \<phi> = local.sat' \<sigma> V5 v i5 \<phi>" for \<phi> V5 i5 
-    using MatchF apply (auto simp add: regex.pred_set fv_regex_alt) 
+    using MatchF apply (auto simp add: regex.pred_set fv_regex_alt) sorry
   then show ?case  using match_cong[OF refl other_IH, where ?r=x2] by auto 
 next
   case (MatchP S E x2 x1)
     from this  have other_IH: "\<phi> \<in> regex.atms x2 \<Longrightarrow> Formula.sat \<sigma> V5 v i5 \<phi> = local.sat' \<sigma> V5 v i5 \<phi>" for \<phi> V5 i5 
-    by (auto simp add: regex.pred_set fv_regex_alt)
+    apply (auto simp add: regex.pred_set fv_regex_alt) sorry
   then show ?case  using match_cong[OF refl other_IH, where ?r=x2] by auto 
 qed  (auto split: nat.splits) 
-  oops
 
+ (* using assms proof (induction arbitrary: v V i S E rule: safe_formula_induct)
+
+  case (Pred e ts)
+  then show ?case sorry
+next
+  case (Let p \<phi> \<psi>)
+  then show ?case sorry
+next
+  case (And_assign \<phi> \<psi>)
+  then show ?case sorry
+next
+  case (And_safe \<phi> \<psi>)
+  then show ?case sorry
+next
+  case (And_constraint \<phi> \<psi>)
+  then show ?case sorry
+next
+  case (And_Not \<phi> \<psi>)
+  then show ?case sorry
+next
+  case (Ands l pos neg)
+  then show ?case sorry
+
+next
+  case (Exists \<phi> t)
+ {
+    fix za
+    assume  assm: "Formula.sat \<sigma> V (za # v) i \<phi>" 
+    from Exists.prems(1) have wty: "S, case_nat t E \<turnstile> \<phi>" by cases
+    have nfv: " Formula.nfv \<phi> \<le> Suc (length v)" using Exists(6) nfv_exists[of \<phi> t] by auto
+    have "0 \<in> fv \<phi> \<Longrightarrow> ty_of za = t" 
+      using ty_of_sat_safe[where ?E="case_nat t E" and ?S=S and ?\<phi>=\<phi> and ?v="za#v" and ?V=V and ?i=i and ?\<sigma>=\<sigma> and ?x=0]  
+      Exists(1,5)  nfv assm wty by auto 
+    then have "\<forall>y\<in>fv \<phi>. ty_of ((za # v) ! y) = (case y of 0 \<Rightarrow> t | Suc x \<Rightarrow> E x)" using  Exists.prems(2)   by (auto simp add:  fvi_Suc split: nat.splits )
+
+    from this  have "local.sat' \<sigma> V (za # v) i \<phi>" using Exists.IH[of S "case_nat t E" "za#v" V i] Exists(5) wty nfv assm by auto
+  }
+  moreover {
+   fix za
+    assume  assm: "sat' \<sigma> V (za # v) i \<phi>" 
+    from Exists.prems(1) have wty: "S, case_nat t E \<turnstile> \<phi>" by cases
+    have nfv: " Formula.nfv \<phi> \<le> Suc (length v)" using Exists(6) nfv_exists[of \<phi> t] by auto
+    have "0 \<in> fv \<phi> \<Longrightarrow> ty_of za = t" 
+      using ty_of_sat'_safe[where ?E="case_nat t E" and ?S=S and ?\<phi>=\<phi> and ?v="za#v" and ?V=V and ?i=i and ?\<sigma>=\<sigma> and ?x=0]  
+      Exists(1,5)  nfv assm wty by auto 
+    then have "\<forall>y\<in>fv \<phi>. ty_of ((za # v) ! y) = (case y of 0 \<Rightarrow> t | Suc x \<Rightarrow> E x)" using  Exists.prems(2)   by (auto simp add:  fvi_Suc split: nat.splits )
+
+    from this  have "Formula.sat \<sigma> V (za # v) i \<phi>" using Exists.IH[of S "case_nat t E" "za#v" V i] Exists(5) wty nfv assm by auto
+  }
+  ultimately show ?case   by auto 
+next
+case (Agg y \<omega> tys f \<phi>)
+  then show ?case sorry
+
+next
+  case (Since \<phi> I \<psi>)
+  then show ?case sorry
+next
+  case (Not_Since \<phi> I \<psi>)
+  then show ?case sorry
+next
+  case (Until \<phi> I \<psi>)
+  then show ?case sorry
+next
+  case (Not_Until \<phi> I \<psi>)
+  then show ?case sorry
+next
+  case (MatchP I r)
+  from this  have other_IH: "\<phi> \<in> regex.atms r \<Longrightarrow> Formula.sat \<sigma> V5 v i5 \<phi> = local.sat' \<sigma> V5 v i5 \<phi>" for \<phi> V5 i5 
+    using MatchP apply (auto simp add: regex.pred_set fv_regex_alt)  sorry
+  then show ?case  using match_cong[OF refl other_IH, where ?r=r] by auto 
+next
+  case (MatchF I r)
+    from this  have other_IH: "\<phi> \<in> regex.atms r \<Longrightarrow> Formula.sat \<sigma> V5 v i5 \<phi> = local.sat' \<sigma> V5 v i5 \<phi>" for \<phi> V5 i5 
+    using MatchF apply (auto simp add: regex.pred_set fv_regex_alt) sorry
+  then show ?case  using match_cong[OF refl other_IH, where ?r=r] by auto
+qed (auto elim: wty_formula.cases split: nat.splits)
+*)
 
 end
 end
