thys/MFODL_Monitor_Devel/Typing.thy
@@ -310,20 +310,182 @@ proof -
         linorder.set_sorted_list_of_set[OF ID_ccompare[OF c]])
 qed
 
-lemma ty_of_sat_safe: "safe_formula \<phi> \<Longrightarrow> S, E \<turnstile> \<phi> \<Longrightarrow> wty_envs S \<sigma> V \<Longrightarrow> 
-  Formula.sat \<sigma> V v i \<phi> \<Longrightarrow> x \<in> Formula.fv \<phi> \<Longrightarrow> Formula.nfv \<phi> \<le> length v \<Longrightarrow> ty_of (v ! x) = E x"
+locale sat_general =
+  fixes 
+undef_plus :: "event_data \<Rightarrow> event_data \<Rightarrow> event_data" and
+undef_minus :: "event_data \<Rightarrow> event_data \<Rightarrow> event_data" and
+undef_uminus :: " event_data \<Rightarrow> event_data" and
+undef_times :: "event_data \<Rightarrow> event_data \<Rightarrow> event_data" and
+undef_divide :: "event_data \<Rightarrow> event_data \<Rightarrow> event_data" and
+undef_modulo :: "event_data \<Rightarrow> event_data \<Rightarrow> event_data"  and
+undef_double_of_event_data :: "event_data \<Rightarrow> double" and
+undef_integer_of_event_data :: "event_data \<Rightarrow> integer" and
+undef_less_eq :: "event_data \<Rightarrow> event_data \<Rightarrow> bool"
+assumes undef_plus_sound:  "\<And>x y. undef_plus (EInt x) (EInt y) = EInt x + EInt y" 
+    "\<And> x y . undef_plus (EFloat x) (EFloat y) = EFloat x + EFloat y"
+assumes undef_minus_sound:  "\<And>x y. undef_minus (EInt x) (EInt y) = EInt x - EInt y" 
+    "\<And> x y . undef_minus (EFloat x) (EFloat y) = EFloat x - EFloat y"
+assumes undef_uminus_sound:  "\<And>x . undef_uminus (EInt x) = - EInt x"
+   "\<And> x. undef_uminus (EFloat x) = - EFloat x "
+assumes undef_times_sound:  "\<And>x y.  undef_times (EInt x) (EInt y) = EInt x * EInt y" 
+    "\<And> x y . undef_times (EFloat x) (EFloat y) = EFloat x * EFloat y"
+assumes undef_divide_sound:  "\<And>x y. undef_divide (EInt x) (EInt y) = EInt x div EInt y" 
+    "\<And> x y .  undef_divide (EFloat x) (EFloat y) = EFloat x div EFloat y"
+assumes undef_modulo_sound:  "\<And>x y.  undef_modulo (EInt x) (EInt y) = EInt x mod EInt y"  
+
+assumes undef_double_of_event_data_sound: "\<And>x.  undef_double_of_event_data (EInt x) = double_of_event_data (EInt x)"
+assumes undef_integer_of_event_data_sound: "\<And>x. undef_integer_of_event_data (EFloat x) = integer_of_event_data (EFloat x)"
+
+assumes undef_less_eq_sound: "\<And>x y. undef_less_eq (EInt x) (EInt y) \<longleftrightarrow> EInt x \<le> EInt y"
+ "\<And>x y. undef_less_eq (EFloat x) (EFloat y) \<longleftrightarrow> EFloat x \<le> EFloat y"
+ "\<And> x y. undef_less_eq (EString x) (EString y) \<longleftrightarrow> EString x \<le> EString y"
+
+begin
+
+definition undef_less :: "event_data \<Rightarrow> event_data \<Rightarrow> bool"  where
+  "undef_less x y \<longleftrightarrow> undef_less_eq x y \<and> \<not> undef_less_eq y x"
+
+definition undef_min :: "event_data \<Rightarrow> event_data \<Rightarrow> event_data" where
+  "undef_min a b = (if undef_less_eq a b then a else b)"
+
+definition undef_max :: "event_data \<Rightarrow> event_data \<Rightarrow> event_data" where
+  "undef_max a b = (if undef_less_eq a b then b else a)"
+
+primrec eval_trm' :: "Formula.env \<Rightarrow> Formula.trm \<Rightarrow> event_data" where
+  "eval_trm' v (Formula.Var x) = v ! x"
+| "eval_trm' v (Formula.Const x) = x"
+| "eval_trm' v (Formula.Plus x y) = undef_plus (eval_trm' v x) ( eval_trm' v y)"
+| "eval_trm' v (Formula.Minus x y) = undef_minus (eval_trm' v x) ( eval_trm' v y)"
+| "eval_trm' v (Formula.UMinus x) = undef_uminus (eval_trm' v x)"
+| "eval_trm' v (Formula.Mult x y) = undef_times (eval_trm' v x) (eval_trm' v y)"
+| "eval_trm' v (Formula.Div x y) = undef_divide (eval_trm' v x) (eval_trm' v y)"
+| "eval_trm' v (Formula.Mod x y) = undef_modulo (eval_trm' v x) (eval_trm' v y)"
+| "eval_trm' v (Formula.F2i x) = EInt (undef_integer_of_event_data (eval_trm' v x))"
+| "eval_trm' v (Formula.I2f x) = EFloat (undef_double_of_event_data (eval_trm' v x))"
+
+
+fun eval_agg_op' :: "Formula.agg_op \<Rightarrow> (event_data \<times> enat) set \<Rightarrow> event_data" where
+  "eval_agg_op' (agg_type.Agg_Cnt, y0) M = (case (flatten_multiset M, finite_multiset M) of
+    (_, False) \<Rightarrow> y0
+    |    ([],_) \<Rightarrow> y0
+    | (xs,_) \<Rightarrow> EInt (integer_of_int (length xs)))"
+| "eval_agg_op' (agg_type.Agg_Min, y0) M = (case  (flatten_multiset M, finite_multiset M) of
+    (_, False) \<Rightarrow> y0
+    |    ([],_) \<Rightarrow> y0
+    | (x # xs,_) \<Rightarrow> foldl undef_min x xs)"
+| "eval_agg_op' (agg_type.Agg_Max, y0) M = (case  (flatten_multiset M, finite_multiset M) of
+    (_, False) \<Rightarrow> y0
+    |    ([],_) \<Rightarrow> y0
+    | (x # xs,_) \<Rightarrow> foldl undef_max x xs)"
+| "eval_agg_op' (agg_type.Agg_Sum, y0) M = (case  (flatten_multiset M, finite_multiset M) of
+    (_, False) \<Rightarrow> y0
+    |    ([],_) \<Rightarrow> y0
+    | (x # xs,_) \<Rightarrow> foldl undef_plus x xs)"
+| "eval_agg_op' (agg_type.Agg_Avg, y0) M =(case  (flatten_multiset M, finite_multiset M) of
+    (_, False) \<Rightarrow> y0
+    |    ([],_) \<Rightarrow> y0
+    | (x#xs,_) \<Rightarrow> EFloat ( undef_double_of_event_data (foldl undef_plus x xs) / double_of_int (length (x#xs))))"
+| "eval_agg_op' (agg_type.Agg_Med, y0) M =(case (flatten_multiset M, finite_multiset M) of
+    (_, False) \<Rightarrow> y0
+    |    ([],_) \<Rightarrow> y0
+    | (xs,_) \<Rightarrow> EFloat (let u = length xs;  u' = u div 2 in
+          if even u then
+            (undef_double_of_event_data (xs ! (u'-1)) + undef_double_of_event_data (xs ! u') / double_of_int 2)
+          else undef_double_of_event_data (xs ! u')))"
+
+fun sat' :: "Formula.trace \<Rightarrow> (Formula.name \<rightharpoonup> nat \<Rightarrow> event_data list set) \<Rightarrow> Formula.env \<Rightarrow> nat \<Rightarrow> 't Formula.formula \<Rightarrow> bool" where
+  "sat' \<sigma> V v i (Formula.Pred r ts) = (case V r of
+       None \<Rightarrow> (r, map (eval_trm' v) ts) \<in> \<Gamma> \<sigma> i
+     | Some X \<Rightarrow> map (eval_trm' v) ts \<in> X i)"
+| "sat' \<sigma> V v i (Formula.Let p \<phi> \<psi>) =
+    sat' \<sigma> (V(p \<mapsto> \<lambda>i. {v. length v = Formula.nfv \<phi> \<and> sat' \<sigma> V v i \<phi>})) v i \<psi>"
+| "sat' \<sigma> V v i (Formula.Eq t1 t2) =  (eval_trm' v t1 = eval_trm' v t2)"
+| "sat' \<sigma> V v i (Formula.Less t1 t2) = undef_less (eval_trm' v t1) (eval_trm' v t2)"
+| "sat' \<sigma> V v i (Formula.LessEq t1 t2) = undef_less_eq (eval_trm' v t1) (eval_trm' v t2)"
+| "sat' \<sigma> V v i (Formula.Neg \<phi>) = (\<not> sat' \<sigma> V v i \<phi>)"
+| "sat' \<sigma> V v i (Formula.Or \<phi> \<psi>) = (sat' \<sigma> V v i \<phi> \<or> sat' \<sigma> V v i \<psi>)"
+| "sat' \<sigma> V v i (Formula.And \<phi> \<psi>) = (sat' \<sigma> V v i \<phi> \<and> sat' \<sigma> V v i \<psi>)"
+| "sat' \<sigma> V v i (Formula.Ands l) = (\<forall>\<phi> \<in> set l. sat' \<sigma> V v i \<phi>)"
+| "sat' \<sigma> V v i (Formula.Exists t \<phi>) = (\<exists>z. sat' \<sigma> V (z # v) i \<phi>)"
+| "sat' \<sigma> V v i (Formula.Agg y \<omega> tys f \<phi>) =
+    (let M = {(x, ecard Zs) | x Zs. Zs = {zs. length zs = length tys \<and> sat' \<sigma> V (zs @ v) i \<phi> \<and> eval_trm' (zs @ v) f = x} \<and> Zs \<noteq> {}}
+    in (M = {} \<longrightarrow> fv \<phi> \<subseteq> {0..< length tys}) \<and> v ! y = eval_agg_op' \<omega> M)"
+| "sat' \<sigma> V v i (Formula.Prev I \<phi>) = (case i of 0 \<Rightarrow> False | Suc j \<Rightarrow> mem I (\<tau> \<sigma> i - \<tau> \<sigma> j) \<and> sat' \<sigma> V v j \<phi>)"
+| "sat' \<sigma> V v i (Formula.Next I \<phi>) = (mem I ((\<tau> \<sigma> (Suc i) - \<tau> \<sigma> i)) \<and> sat' \<sigma> V v (Suc i) \<phi>)"
+| "sat' \<sigma> V v i (Formula.Since \<phi> I \<psi>) = (\<exists>j\<le>i. mem I (\<tau> \<sigma> i - \<tau> \<sigma> j) \<and> sat' \<sigma> V v j \<psi> \<and> (\<forall>k \<in> {j <.. i}. sat' \<sigma> V v k \<phi>))"
+| "sat' \<sigma> V v i (Formula.Until \<phi> I \<psi>) = (\<exists>j\<ge>i. mem I (\<tau> \<sigma> j - \<tau> \<sigma> i) \<and> sat' \<sigma> V v j \<psi> \<and> (\<forall>k \<in> {i ..< j}. sat' \<sigma> V v k \<phi>))"
+| "sat' \<sigma> V v i (Formula.MatchP I r) = (\<exists>j\<le>i. mem I (\<tau> \<sigma> i - \<tau> \<sigma> j) \<and> Regex.match (sat' \<sigma> V v) r j i)"
+| "sat' \<sigma> V v i (Formula.MatchF I r) = (\<exists>j\<ge>i. mem I (\<tau> \<sigma> j - \<tau> \<sigma> i) \<and> Regex.match (sat' \<sigma> V v) r i j)"
+
+
+
+lemma eval_trm_sound: 
+  assumes "E \<turnstile> f :: t"  "\<forall>y\<in>fv_trm f. ty_of (v ! y) = E y"
+  shows "Formula.eval_trm v f = eval_trm' v f"
+  using assms  
+  apply  (induction  rule: wty_trm.induct) apply (auto simp add: numeric_ty_def)
+  subgoal for x y  using  value_of_eval_trm[of E x v] value_of_eval_trm[of E y v] by (auto simp add: undef_plus_sound)
+    subgoal for x y  using  value_of_eval_trm[of E x v] value_of_eval_trm[of E y v] by (auto simp add: undef_plus_sound)
+  subgoal for x y
+    using  value_of_eval_trm[of E x v] value_of_eval_trm[of E y v] by (auto simp add: undef_minus_sound) 
+ subgoal for x y
+   using  value_of_eval_trm[of E x v] value_of_eval_trm[of E y v] by (auto simp add: undef_minus_sound)
+ subgoal for x 
+   using  value_of_eval_trm[of E x v]  by (auto simp add: undef_uminus_sound)
+ subgoal for x 
+   using  value_of_eval_trm[of E x v]  by (auto simp add: undef_uminus_sound)
+  subgoal for x y  using  value_of_eval_trm[of E x v] value_of_eval_trm[of E y v] by (auto simp add: undef_times_sound)
+  subgoal for x y  using  value_of_eval_trm[of E x v] value_of_eval_trm[of E y v] by (auto simp add: undef_times_sound)
+  subgoal for x y  using  value_of_eval_trm[of E x v] value_of_eval_trm[of E y v] by (auto simp add: undef_divide_sound)
+  subgoal for x y  using  value_of_eval_trm[of E x v] value_of_eval_trm[of E y v] by (auto simp add: undef_divide_sound)
+  subgoal for x y  using  value_of_eval_trm[of E x v] value_of_eval_trm[of E y v] by (auto simp add: undef_modulo_sound)
+  subgoal for x  using  value_of_eval_trm[of E x v] by (auto simp add: undef_integer_of_event_data_sound)
+  subgoal for x  using  value_of_eval_trm[of E x v] by (auto simp add: undef_double_of_event_data_sound)
+  done
+
+lemma nfv_exists: " Formula.nfv \<phi> \<le> Suc (Formula.nfv (Formula.Exists t \<phi>))"
+   apply (auto simp add: Formula.nfv_def fvi_Suc) 
+  by (metis Max.coboundedI finite_fvi finite_imageI finite_insert fvi_Suc imageI insertCI list_decode.cases)
+
+lemma match_sat'_fv: assumes "safe_regex temp Strict r"
+    "Regex.match (sat' \<sigma> V v) r j i"
+    "x \<in> fv (formula.MatchP I r) \<or> x \<in>fv (formula.MatchF I r)"
+  shows "\<exists>\<phi>\<in>atms r. \<exists>k. sat' \<sigma> V v k \<phi> \<and> x \<in> fv \<phi>"
+  using assms
+  proof (induction r arbitrary:i j)
+
+    case (Plus r1 r2)
+  moreover obtain k where "\<exists>j. Regex.match (sat' \<sigma> V v) r1 j k \<or>  Regex.match (sat' \<sigma> V v) r2 j k" using  Plus.prems(2)  by auto
+  moreover {
+    assume assm: "\<exists>j. Regex.match (sat' \<sigma> V v) r1 j k"
+    then have ?case using Plus.prems(1,3) Plus.IH(1)  by (fastforce simp add: atms_def) 
+  } moreover {
+    assume assm: "\<exists>j. Regex.match (sat' \<sigma> V v) r2 j k"
+    from this have ?case using Plus.prems(1,3) Plus.IH(2) by (fastforce simp add: atms_def)
+  }
+  ultimately show ?case by auto
+next
+  case (Times r1 r2)
+  then show ?case  using Times.prems match_le Times.IH  by (cases temp) fastforce+
+qed  auto
+
+
+
+lemma ty_of_sat'_safe: "safe_formula \<phi> \<Longrightarrow> S, E \<turnstile> \<phi> \<Longrightarrow> wty_envs S \<sigma> V \<Longrightarrow> 
+  sat' \<sigma> V v i \<phi> \<Longrightarrow> x \<in> Formula.fv \<phi> \<Longrightarrow> Formula.nfv \<phi> \<le> length v \<Longrightarrow> ty_of (v ! x) = E x"
 proof (induction arbitrary: S E V v i x rule: safe_formula_induct)
   case (Eq_Const c d)
   then show ?case by auto
 next
   case (Eq_Var1 c xa)
+   case (Eq_Var1 c xa)
   from Eq_Var1.prems(1) obtain t where 
 " E \<turnstile> (trm.Const c) :: t" and "E \<turnstile> (trm.Var xa) :: t"
     by cases
   from Eq_Var1(4)  have "x = xa" by auto
   from this `E \<turnstile> (trm.Var xa) :: t` have "E x = t" using  wty_trm.cases by fastforce
-  from this Eq_Var1 ` E \<turnstile> (trm.Const c) :: t` show ?case 
-    by (metis \<open>x = xa\<close> empty_iff eval_trm.simps(1) fvi_trm.simps(2) sat.simps(3) ty_of_eval_trm)
+  from this Eq_Var1 ` E \<turnstile> (trm.Const c) :: t` show ?case
+    by (metis \<open>x = xa\<close> empty_iff eval_trm'.simps(1) fvi_trm.simps(2) sat'.simps(3) eval_trm_sound ty_of_eval_trm)
 
 next
   case (Eq_Var2 c xa)
@@ -333,18 +495,18 @@ next
   from Eq_Var2(4)  have "x = xa" by auto
   from this `E \<turnstile> (trm.Var xa) :: t` have "E x = t" using  wty_trm.cases by fastforce
   from this Eq_Var2 ` E \<turnstile> (trm.Const c) :: t` show ?case
-    by (metis \<open>x = xa\<close> empty_iff eval_trm.simps(1) fvi_trm.simps(2) sat.simps(3) ty_of_eval_trm)
+    by (metis \<open>x = xa\<close> empty_iff eval_trm'.simps(1) fvi_trm.simps(2) sat'.simps(3) eval_trm_sound ty_of_eval_trm)
   
 next
   case (neq_Var xa)
-  thus ?case by auto
+  thus ?case by (auto) 
 next
   case (Pred p tms)
   from Pred.prems(1) obtain tys where
     S_p: "S p = Some tys" and
     xs_ts: "list_all2 (\<lambda>tm ty. E \<turnstile> tm :: ty) tms tys"
     by cases
-  let ?xs = "map (Formula.eval_trm v) tms"
+  let ?xs = "map (eval_trm' v) tms"
   have wty_xs: "wty_tuple tys ?xs"
   proof (cases "p \<in> dom V")
     case True
@@ -370,7 +532,7 @@ next
   finally show ?case .
 next
   case (Let p \<phi> \<psi>)
-  let ?V' = "V(p \<mapsto> \<lambda>i. {v. length v = Formula.nfv \<phi> \<and> Formula.sat \<sigma> V v i \<phi>})"
+  let ?V' = "V(p \<mapsto> \<lambda>i. {v. length v = Formula.nfv \<phi> \<and> sat' \<sigma> V v i \<phi>})"
   from Let.prems(1) obtain E' where
     wty_\<phi>: "S, E' \<turnstile> \<phi>" and
     wty_\<psi>: "S(p \<mapsto> tabulate E' 0 (Formula.nfv \<phi>)), E \<turnstile> \<psi>"
@@ -378,21 +540,21 @@ next
   let ?tys = "tabulate E' 0 (Formula.nfv \<phi>)"
   {
     fix v' i
-    assume "length v' = Formula.nfv \<phi>" and "Formula.sat \<sigma> V v' i \<phi>"
+    assume "length v' = Formula.nfv \<phi>" and "sat' \<sigma> V v' i \<phi>"
     then have "wty_tuple ?tys v'"
       using Let.IH(1) wty_\<phi> Let.prems(2) Let.hyps(1)
       by (auto simp: wty_tuple_def list_all2_conv_all_nth)
   }
   with Let.prems(2) have "wty_envs (S(p \<mapsto> ?tys)) \<sigma> ?V'"
     by (auto simp: wty_envs_def wty_event_def)
-  from Let.prems(3) have "Formula.sat \<sigma> ?V' v i \<psi>" by simp
+  from Let.prems(3) have "sat' \<sigma> ?V' v i \<psi>" by simp
   from Let.prems(4) have "x \<in> fv \<psi>" by simp
   from Let have "Formula.nfv \<psi> \<le> length v" by auto
   show ?case by (rule Let.IH(2)) fact+
 next
   case (And_assign \<phi> \<psi>)
   from And_assign.prems(1) have phi1: "S, E \<turnstile> \<phi>" by cases
-  from And_assign.prems(3) have phi2: "Formula.sat \<sigma> V v i \<psi>" by auto
+  from And_assign.prems(3) have phi2: "sat' \<sigma> V v i \<psi>" by auto
   from And_assign.prems(4) have "x \<in> fv \<phi> \<or> x \<in> fv \<psi>" by auto
   from this show ?case
   proof cases
@@ -406,22 +568,22 @@ next
     moreover {
       assume a_def: "a = Formula.Var x"
       from this  x_not_\<phi> have fvb: "fv_trm b \<subseteq> fv \<phi>" using And_assign(2) by  (auto simp: safe_assignment_def \<psi>_eq split: trm.splits) 
-      have eval:" v! x = Formula.eval_trm v b" using And_assign(6) a_def \<psi>_eq by auto
+      have eval:" v! x = eval_trm' v b" using And_assign(6) a_def \<psi>_eq by auto
       have Ebx: "E \<turnstile> b :: E  x"  using And_assign(4) by (auto simp: \<psi>_eq a_def elim: wty_trm.cases wty_formula.cases)
       have "(\<lambda>y. ty_of (v ! y)) \<turnstile> b :: E x" apply (rule  iffD1[OF wty_trm_fv_cong,OF _ Ebx]) apply (subst eq_commute) 
         apply (rule And_assign(3)) using And_assign fvb by (auto elim: wty_formula.cases) 
       then have ?case using ty_of_eval_trm unfolding eval
-        using And_assign(4) by (auto simp: \<psi>_eq a_def elim: wty_formula.cases)
+        using And_assign(4) by (auto simp: \<psi>_eq a_def eval_trm_sound elim: wty_formula.cases)
     }
     moreover {
      assume a_def: "b = Formula.Var x"
       from this  x_not_\<phi> have fvb: "fv_trm a \<subseteq> fv \<phi>" using And_assign(2) by  (auto simp: safe_assignment_def \<psi>_eq split: trm.splits) 
-      have eval:" v! x = Formula.eval_trm v a" using And_assign(6) a_def \<psi>_eq by auto
+      have eval:" v! x = eval_trm' v a" using And_assign(6) a_def \<psi>_eq by auto
       have Ebx: "E \<turnstile> a :: E  x"  using And_assign(4) by (auto simp: \<psi>_eq a_def elim: wty_trm.cases wty_formula.cases)
       have "(\<lambda>y. ty_of (v ! y)) \<turnstile> a :: E x" apply (rule  iffD1[OF wty_trm_fv_cong,OF _ Ebx]) apply (subst eq_commute) 
         apply (rule And_assign(3)) using And_assign fvb by (auto elim: wty_formula.cases) 
       then have ?case using ty_of_eval_trm unfolding eval
-        using And_assign(4) by (auto simp: \<psi>_eq a_def elim: wty_formula.cases)
+        using And_assign(4)  by (auto simp: \<psi>_eq a_def eval_trm_sound elim: wty_formula.cases)
     }
     moreover
       have "a = Formula.Var x \<or> b = Formula.Var x" using And_assign(2) And_assign(7) x_not_\<phi> by (auto simp: \<psi>_eq safe_assignment_def split: Formula.trm.splits) 
@@ -430,7 +592,7 @@ qed
  next
   case (And_safe \<phi> \<psi>)
   from And_safe.prems(1) obtain "S, E \<turnstile> \<phi>" and "S, E \<turnstile> \<psi>" by cases
-  from And_safe.prems(3) have "Formula.sat \<sigma> V v i \<phi>" and "Formula.sat \<sigma> V v i \<psi>"
+  from And_safe.prems(3) have "sat' \<sigma> V v i \<phi>" and "sat' \<sigma> V v i \<psi>"
     by simp_all
   from And_safe.prems(4) consider (in_\<phi>) "x \<in> fv \<phi>" | (in_\<psi>) "x \<in> fv \<psi>" by auto
   then show ?case
@@ -471,11 +633,11 @@ next
   from this Ands(1) have phi_in_l: "\<phi> \<in> set l" by auto
   from phidef Ands(6) have phi_IH: "S, E \<turnstile> \<phi> \<Longrightarrow>
     wty_envs S \<sigma> V \<Longrightarrow>
-    Formula.sat \<sigma> V v i \<phi> \<Longrightarrow> x \<in> fv \<phi> \<Longrightarrow> Formula.nfv \<phi> \<le> length v \<Longrightarrow> ty_of (v ! x) = E x"
+    sat' \<sigma> V v i \<phi> \<Longrightarrow> x \<in> fv \<phi> \<Longrightarrow> Formula.nfv \<phi> \<le> length v \<Longrightarrow> ty_of (v ! x) = E x"
         using list_all2_iff by (smt (verit, ccfv_SIG) Ball_set_list_all)
       from Ands.prems(1) have  "\<forall>\<phi> \<in> set l. S, E \<turnstile> \<phi>" by cases
       from this phi_in_l have p1: "S, E \<turnstile> \<phi>"  by auto
-      from phi_in_l Ands.prems(3) have p3: "Formula.sat \<sigma> V v i \<phi>" by auto
+      from phi_in_l Ands.prems(3) have p3: "sat' \<sigma> V v i \<phi>" by auto
       from phi_in_l Ands have p5: "Formula.nfv \<phi> \<le> length v" by auto
   from  phi_IH p1 Ands.prems(2) p3 phidef p5  show ?case by auto
 next
@@ -483,15 +645,15 @@ next
   from Neg show ?case by auto
 next
   case (Or \<phi> \<psi>)
-  from Or.prems(3) have " (Formula.sat \<sigma> V v i \<phi>) \<or>( Formula.sat \<sigma> V v i \<psi>)" by auto
+  from Or.prems(3) have " (sat' \<sigma> V v i \<phi>) \<or>( sat' \<sigma> V v i \<psi>)" by auto
   from this show ?case 
   proof
-    assume assm: "(Formula.sat \<sigma> V v i \<phi>)"
+    assume assm: "(sat' \<sigma> V v i \<phi>)"
   from Or(1) Or.prems(4) have xfv: "x \<in> fv \<phi>" by auto
   from Or.prems(1) have "S, E \<turnstile> \<phi>" by cases
   from this assm Or.prems(2,3) Or(4) Or.prems(5) xfv show ?case by auto
 next 
-  assume assm: "( Formula.sat \<sigma> V v i \<psi>)"
+  assume assm: "( sat' \<sigma> V v i \<psi>)"
  from Or(1) Or.prems(4) have xfv: "x \<in> fv \<psi>" by auto
   from Or.prems(1) have "S, E \<turnstile> \<psi>" by cases
   from this assm Or.prems(2,3) Or(5) Or.prems(5) xfv show ?case by auto
@@ -499,7 +661,7 @@ qed
 next
   case (Exists \<phi>)
   from Exists.prems(1) obtain t where "S, case_nat t E \<turnstile> \<phi>" by cases
-  from Exists.prems(3) obtain z where "Formula.sat \<sigma> V (z#v) i \<phi>" by auto
+  from Exists.prems(3) obtain z where "sat' \<sigma> V (z#v) i \<phi>" by auto
   from Exists.prems(4) have "Suc x \<in> fv \<phi>" by (simp add: fvi_Suc)
   from Exists have "Formula.nfv \<phi> \<le> Suc (length v)" apply (auto simp add: Formula.nfv_def)
     by (metis fvi_Suc le0 old.nat.exhaust)
@@ -520,8 +682,8 @@ next
     assume asm: "x \<in> Formula.fvi (length tys) \<phi>"
     from this have "\<not> fv \<phi> \<subseteq> {0..< length tys}" using fvi_iff_fv[of x "length tys" \<phi>] by auto
     from this have M: "{(x, ecard Zs) | 
-  x Zs. Zs = {zs. length zs = length tys \<and> Formula.sat \<sigma> V (zs @ v) i \<phi> \<and> Formula.eval_trm (zs @ v) f = x} \<and> Zs \<noteq> {}} \<noteq> {}" using Agg.prems(3) by auto
-    from this obtain zs where sat: "Formula.sat \<sigma> V (zs @ v) i \<phi> \<and> length zs = length tys" by auto
+  x Zs. Zs = {zs. length zs = length tys \<and> sat' \<sigma> V (zs @ v) i \<phi> \<and> eval_trm' (zs @ v) f = x} \<and> Zs \<noteq> {}} \<noteq> {}" using Agg.prems(3) by auto
+    from this obtain zs where sat: "sat' \<sigma> V (zs @ v) i \<phi> \<and> length zs = length tys" by auto
     from nfv_tys_v have nfv: "Formula.nfv \<phi> \<le> length (zs @ v)"  by (auto simp add: sat)
     have "ty_of ((zs@v) ! (x + length tys)) = agg_env E tys (x + length tys)"
       apply (rule Agg.IH[of \<phi> S "agg_env E tys" V "zs @ v" i "x+ length tys"]) using Agg.prems(1) Agg(4) sat asm nfv Agg.prems(1-2) fvi_iff_fv
@@ -536,73 +698,89 @@ next
     from this eq obtain t where t_def: "E x = t_res agg_type t" by blast
     from  Agg.prems(1) have
  ty_of_d: "ty_of d = t_res agg_type t" apply cases using eq omega_def t_def by auto
-    from Agg.prems(3) eq obtain M where  M_def: "M = {(x, ecard Zs) | x Zs. Zs = {zs. length zs = length tys \<and> Formula.sat \<sigma> V (zs @ v) i \<phi>
-        \<and> Formula.eval_trm (zs @ v) f = x} \<and> Zs \<noteq> {}} \<and> v!x = eval_agg_op \<omega> M" by auto
+    from Agg.prems(3) eq obtain M where  M_def: "M = {(x, ecard Zs) | x Zs. Zs = {zs. length zs = length tys \<and> sat' \<sigma> V (zs @ v) i \<phi>
+        \<and> eval_trm' (zs @ v) f = x} \<and> Zs \<noteq> {}} \<and> v!x = eval_agg_op' \<omega> M" by auto
    
         {
            assume finite_M: "finite_multiset M"
-    from this   have finite_set:"finite {x. {zs. length zs = length tys \<and> Formula.sat \<sigma> V (zs @ v) i \<phi> \<and> Formula.eval_trm (zs @ v) f = x} \<noteq> {}}"
+    from this   have finite_set:"finite {x. {zs. length zs = length tys \<and> sat' \<sigma> V (zs @ v) i \<phi> \<and> eval_trm' (zs @ v) f = x} \<noteq> {}}"
        using finite_fst by (auto simp add: finite_multiset_def M_def ) 
     have flatten: "set (flatten_multiset M) \<subseteq> fst ` M" using finite_set  set_of_flatten_multiset[of M
- "(\<lambda>x . {zs . length zs = length tys \<and> Formula.sat \<sigma> V (zs @ v) i \<phi> \<and> Formula.eval_trm (zs @ v) f = x} )"]
+ "(\<lambda>x . {zs . length zs = length tys \<and> sat' \<sigma> V (zs @ v) i \<phi> \<and> eval_trm' (zs @ v) f = x} )"]
        by (auto simp add:  M_def) 
-    from this  have evaltrm: "z \<in> set (flatten_multiset M) \<Longrightarrow>  \<exists> zs. length zs = length tys \<and> Formula.sat \<sigma> V (zs @ v) i \<phi> \<and> Formula.eval_trm (zs @ v) f = z" 
+    from this  have evaltrm: "z \<in> set (flatten_multiset M) \<Longrightarrow>  \<exists> zs. length zs = length tys \<and> sat' \<sigma> V (zs @ v) i \<phi> \<and> eval_trm' (zs @ v) f = z" 
       for z using  M_def by (auto simp add: image_def)
      have th2: ?case if minmaxsum: "agg_type = agg_type.Agg_Min \<or> agg_type = agg_type.Agg_Max \<or> agg_type = agg_type.Agg_Sum" and alist_def: " flatten_multiset
-     {(x, ecard {zs. length zs = length tys \<and> Formula.sat \<sigma> V (zs @ v) i \<phi> \<and> Formula.eval_trm (zs @ v) f = x}) |x.
-      \<exists>xa. Formula.sat \<sigma> V (xa @ v) i \<phi> \<and> length xa = length tys \<and> Formula.eval_trm (xa @ v) f = x} =
+     {(x, ecard {zs. length zs = length tys \<and> sat' \<sigma> V (zs @ v) i \<phi> \<and> eval_trm' (zs @ v) f = x}) |x.
+      \<exists>xa. sat' \<sigma> V (xa @ v) i \<phi> \<and> length xa = length tys \<and> eval_trm' (xa @ v) f = x} =
     a # list"  for a list
      proof -
-      have ty_of_list: "z=a \<or> z \<in> set list \<Longrightarrow> \<exists>zs .ty_of (Formula.eval_trm (zs @ v) f) = t \<and> ty_of z = t" for z
+      have ty_of_list: "z=a \<or> z \<in> set list \<Longrightarrow> \<exists>zs .ty_of (eval_trm' (zs @ v) f) = t \<and> ty_of z = t" for z
       proof -
           assume z_def: "z=a \<or> z \<in> set list"
-        from z_def obtain zs where zs_def: " length zs = length tys \<and> Formula.sat \<sigma> V (zs @ v) i \<phi> \<and> Formula.eval_trm (zs @ v) f = z" using alist_def evaltrm M_def by auto
+        from z_def obtain zs where zs_def: " length zs = length tys \<and> sat' \<sigma> V (zs @ v) i \<phi> \<and> eval_trm' (zs @ v) f = z" using alist_def evaltrm M_def by auto
         from Agg.prems(1) have wty_f: " agg_env E tys  \<turnstile> f :: t" apply cases  using omega_def t_def minmaxsum eq  by auto  
         have fv_ty:"\<forall>y\<in>fv_trm f. ty_of ((zs @ v) ! y) = agg_env E tys y"
         proof 
           fix y
           assume assm: "y \<in> fv_trm f"
-          have  sat: "Formula.sat \<sigma> V (zs @ v) i \<phi>"  using zs_def by auto 
+          have  sat: "sat' \<sigma> V (zs @ v) i \<phi>"  using zs_def by auto 
           show "ty_of ((zs @ v) ! y) = agg_env E tys y" using zs_def assm Agg(3,4) Agg.prems(1-2) nfv_tys_v sat  Agg.IH[of \<phi> S "agg_env E tys" V "zs@v" i y]
             by (auto elim: wty_formula.cases)
         qed      
-        have ty_of_z: "ty_of (Formula.eval_trm (zs @ v) f) = t" using wty_f fv_ty   ty_of_eval_trm[of "agg_env E tys" f t "zs@v" ]
-          by auto
+        have ty_of_z: "ty_of (eval_trm' (zs @ v) f) = t" using wty_f fv_ty   ty_of_eval_trm[of "agg_env E tys" f t "zs@v" ]
+          by (auto simp add: eval_trm_sound)
         from this zs_def show  ?thesis by auto
       qed 
-      from this obtain zs where zs_def: "ty_of (Formula.eval_trm (zs @ v) f) = t" by auto
+      from this obtain zs where zs_def: "ty_of (eval_trm' (zs @ v) f) = t" by auto
       from ty_of_list have indass: "ty_of a = t \<and> (\<forall>z \<in> set list . ty_of z = t)" by auto
      
       from this have foldl_evaltrm: "foldfun = min \<or> foldfun = max
-        \<Longrightarrow> ty_of (foldl foldfun a list) = ty_of (Formula.eval_trm (zs @ v) f)" for foldfun using indass 
+        \<Longrightarrow> ty_of (foldl foldfun a list) = ty_of (eval_trm' (zs @ v) f)" for foldfun using indass 
           proof  (induction list arbitrary: a foldfun)
             case Nil
             then show ?case using zs_def by auto
           next
             case (Cons aa tail)
-             have minmax: " ty_of (foldl foldfun (foldfun a aa) tail) = ty_of (Formula.eval_trm (zs @ v) f)"
+             have minmax: " ty_of (foldl foldfun (foldfun a aa) tail) = ty_of (eval_trm' (zs @ v) f)"
               using Cons.IH[of _ "foldfun a aa"] Cons apply auto 
                apply (metis min_def) by (metis max_def) 
               then show ?case by auto
             qed
 
           from indass have foldl_evaltrm_Sum: 
-              "t \<in> numeric_ty \<Longrightarrow> ty_of (foldl (+) a list) = ty_of (Formula.eval_trm (zs@v) f)" 
+              "t \<in> numeric_ty \<Longrightarrow> ty_of (foldl undef_plus a list) = ty_of (eval_trm' (zs@v) f)" 
               proof (induction list arbitrary: a)
-                case Nil
-                  then show ?case using zs_def by auto
-                next
                   case (Cons aa tail)
-            from this have "ty_of (a + aa) = t"  by (cases aa) ( auto simp add: numeric_ty_def ty_of_plus)
-                  then show ?case using Cons.prems(1) Cons.IH[of "a+aa"] apply auto 
+                  from this have "ty_of (undef_plus a aa) = t"  apply (cases aa)  apply ( auto simp add: numeric_ty_def ty_of_plus)
+                     apply (cases a) apply (auto simp add: undef_plus_sound)
+                    by (cases a)(auto simp add: undef_plus_sound)
+
+                  then show ?case using Cons.prems(1) Cons.IH[of "undef_plus a aa"] apply auto 
                     by (metis Cons.prems(2) list.set_intros(2))
-              qed
+                qed (auto simp add: zs_def)
+
+ from indass have foldl_evaltrm_Min: 
+              " ty_of (foldl undef_min a list) = t" 
+              proof (induction list arbitrary: a)
+                  case (Cons aa tail)
+            from this have "ty_of (undef_min a aa) = t"  apply (cases aa) by ( auto simp add: numeric_ty_def undef_min_def undef_less_eq_sound)
+                  then show ?case using Cons.prems(1) Cons.IH[of "undef_min a aa"] by auto 
+                qed auto
+
+ from indass have foldl_evaltrm_Max: 
+              " ty_of (foldl undef_max a list) = t" 
+              proof (induction list arbitrary: a)
+                  case (Cons aa tail)
+            from this have "ty_of (undef_max a aa) = t"  apply (cases aa) by ( auto simp add: numeric_ty_def undef_max_def undef_less_eq_sound)
+                  then show ?case using Cons.prems(1) Cons.IH[of "undef_max a aa"] by auto 
+              qed auto
            from Agg.prems(1) t_def eq omega_def have num_ty: "agg_type = agg_type.Agg_Sum \<Longrightarrow> t \<in> numeric_ty" by cases auto
          
     
-            from  num_ty  finite_M foldl_evaltrm foldl_evaltrm_Sum  show  ?thesis apply (cases agg_type)
+            from  num_ty  finite_M foldl_evaltrm foldl_evaltrm_Sum foldl_evaltrm_Min foldl_evaltrm_Max show  ?thesis apply (cases agg_type)
                by (auto simp add: M_def  alist_def omega_def finite_multiset_def   
-                      t_def zs_def  split: list.splits) 
+                      t_def zs_def   split: list.splits) 
    
          qed
           from  finite_M th2  M_def t_def omega_def  have ?case apply (cases agg_type) 
@@ -618,11 +796,11 @@ next
   } 
   ultimately show ?case by auto
 next
+  
   case (Prev I \<phi>)
-  from Prev.prems(1) have wty: "S, E \<turnstile> \<phi>" by cases
-  from Prev.prems(3) have forall_j: "\<forall>j . i = Suc j \<longrightarrow> Formula.sat \<sigma> V v j \<phi>" by auto
-  from this have " Formula.sat \<sigma> V v (Nat.pred i) \<phi>" using Prev.prems(3)
-    by (auto split: nat.splits)
+   from Prev.prems(1) have wty: "S, E \<turnstile> \<phi>" by cases
+  from Prev.prems(3) have forall_j: "\<forall>j . i = Suc j \<longrightarrow> sat' \<sigma> V v j \<phi>" by auto
+  from this have "sat' \<sigma> V v (Nat.pred i) \<phi>" using Prev.prems by (auto split: nat.splits)
   from this wty Prev.prems(2-5) Prev.IH show ?case by auto
 next
   case (Next I \<phi>)
@@ -647,34 +825,35 @@ next
   from this wty Not_Until.prems(2-5) Not_Until.IH show ?case by auto
 next
   case (MatchP I r)
-  from MatchP.prems(3) have "(\<exists>j. Regex.match (Formula.sat \<sigma> V v) r j i)" by auto
-    from this  MatchP(1)  MatchP.prems(4) obtain \<phi> j where phidef: " \<phi> \<in> atms r" " Formula.sat \<sigma> V v j \<phi>" "x \<in> fv \<phi> " using match_sat_fv  by auto blast
+  from MatchP.prems(3) have "(\<exists>j. Regex.match (sat' \<sigma> V v) r j i)" by auto
+    from this  MatchP(1)  MatchP.prems(4) obtain \<phi> j where phidef: " \<phi> \<in> atms r" " sat' \<sigma> V v j \<phi>" "x \<in> fv \<phi> " using match_sat'_fv  by auto blast
     have "\<forall>a \<in> fv \<phi>. a \<in> fv_regex r" using   phidef(1)  apply (induction r) apply auto 
       subgoal for \<psi>  apply (cases "safe_formula \<psi>") apply auto by (cases \<psi>) auto 
       done
     from  this MatchP.prems(4,5) phidef  have nfv: "Formula.nfv \<phi> \<le> length v"  by  (auto simp add: Formula.nfv_def)
     from MatchP.IH MatchP.prems have IH: "S, E \<turnstile> \<phi> \<Longrightarrow>\<phi> \<in> atms r \<Longrightarrow>
-     Formula.sat \<sigma> V v j \<phi> \<Longrightarrow> x \<in> fv \<phi> \<Longrightarrow> Formula.nfv \<phi> \<le> length v \<Longrightarrow> ty_of (v ! x ) = E x"
+     sat' \<sigma> V v j \<phi> \<Longrightarrow> x \<in> fv \<phi> \<Longrightarrow> Formula.nfv \<phi> \<le> length v \<Longrightarrow> ty_of (v ! x ) = E x"
     for \<phi> E  v  x by blast
    from MatchP.prems(1) MatchP(1) have  "S, E \<turnstile> \<phi>" using  Regex.Regex.regex.pred_set[of "(\<lambda>\<phi>. S, E \<turnstile> \<phi>)"] phidef(1) wty_regexatms_atms  by cases auto
   then show ?case apply (rule IH) using nfv  MatchP.prems(5) phidef by auto
  
 next
   case (MatchF I r)
- from MatchF.prems(3) have "(\<exists>j. Regex.match (Formula.sat \<sigma> V v) r  i j)" by auto
-    from this  MatchF(1)  MatchF.prems(4) obtain \<phi> j where phidef: " \<phi> \<in> atms r" " Formula.sat \<sigma> V v j \<phi>" "x \<in> fv \<phi> " using match_sat_fv  by auto blast
+ from MatchF.prems(3) have "(\<exists>j. Regex.match (sat' \<sigma> V v) r  i j)" by auto
+    from this  MatchF(1)  MatchF.prems(4) obtain \<phi> j where phidef: " \<phi> \<in> atms r" " sat' \<sigma> V v j \<phi>" "x \<in> fv \<phi> " using match_sat'_fv  by auto blast
     have "\<forall>a \<in> fv \<phi>. a \<in> fv_regex r" using   phidef(1)  apply (induction r) apply auto 
       subgoal for \<psi>  apply (cases "safe_formula \<psi>") apply auto by (cases \<psi>) auto 
       done
     from  this MatchF.prems(4,5) phidef  have nfv: "Formula.nfv \<phi> \<le> length v"  by  (auto simp add: Formula.nfv_def)
     from MatchF.IH MatchF.prems have IH: "S, E \<turnstile> \<phi> \<Longrightarrow>\<phi> \<in> atms r \<Longrightarrow>
-     Formula.sat \<sigma> V v j \<phi> \<Longrightarrow> x \<in> fv \<phi> \<Longrightarrow> Formula.nfv \<phi> \<le> length v \<Longrightarrow> ty_of (v ! x ) = E x"
+     sat' \<sigma> V v j \<phi> \<Longrightarrow> x \<in> fv \<phi> \<Longrightarrow> Formula.nfv \<phi> \<le> length v \<Longrightarrow> ty_of (v ! x ) = E x"
     for \<phi> E  v  x by blast
     from MatchF.prems(1) MatchF(1) have  "S, E \<turnstile> \<phi>" using  Regex.Regex.regex.pred_set[of "(\<lambda>\<phi>. S, E \<turnstile> \<phi>)"] phidef(1) wty_regexatms_atms  by cases auto
   then show ?case apply (rule IH) using nfv  MatchF.prems(5)  phidef by auto
 
 qed
 
+end
 
 (*<*)
 end
